\documentclass{article}
\usepackage[utf8]{inputenc}
\usepackage{graphics}
\usepackage{amsmath}
\usepackage{amssymb}
\usepackage{cases}
\title{Assignment2}
\author{Aditya Gangula EP20BTECH11001}

\begin{document}

\maketitle

\section*{Problem 2.25a}
Let the signal 
\[y[n] = x[n]*h[n]\]
where
\[x[n] = 3^nu[-n-1] + \left(\frac{1}{3}\right)^nu[n]\]
and
\[h[n] = \left(\frac{1}{4}\right)^nu[n+3]\]
Determine $y[n]$ without using the distributive property of convolution.

\raggedright \textbf {Solution:}

$u[-n-1]$ will only be non-zero for $n\leq-1$
\[\therefore x[n] = \left(\frac{1}{3}\right)^{|n|}\]
\[y[n] = \sum_{k=-\infty}^\infty x[k]h[n-k]\]
\[=\sum_{k=-\infty}^\infty \left(\frac{1}{3}\right)^{|k|}\left(\frac{1}{4}\right)^{n-k}u[n-k+3]\]
\[=\sum_{k=0}^\infty \left(\frac{1}{3}\right)^{k}\left(\frac{1}{4}\right)^{n-k}u[n-k+3] + \sum_{k=-\infty}^{-1} \left(\frac{1}{3}\right)^{-k}\left(\frac{1}{4}\right)^{n-k}u[n-k+3]\]
\[=\sum_{k=0}^\infty \left(\frac{1}{3}\right)^{k}\left(\frac{1}{4}\right)^{n-k}u[n-k+3] + \frac{1}{12}\sum_{k=0}^{\infty} \left(\frac{1}{3}\right)^{k}\left(\frac{1}{4}\right)^{n+k}u[n+k+4]\]
using summation of geometric progression formulae we can say that,
\[\implies y(n) = 
\begin{cases}
    \frac{1}{4^n.11} + \frac{4^4}{3^{n-1}} - \frac{3}{4^n} & n \geq -3
    \\
    \frac{4^4}{11} & n=-4
    \\
    \frac{12^4.3^n}{11} & n < -4
\end{cases}
\]
\end{document}
